More work towards the controller proof

Hybrid_Programs/Verification_Examples/Obstacle_Avoidance.thy
@@ -1,6 +1,34 @@
 theory Obstacle_Avoidance
-  imports "Hybrid-Verification.Hybrid_Verification"
+  imports "Hybrid-Verification.Hybrid_Verification" (* "Explorer.Explorer" *)
 begin
+
+(* setup Explorer_Lib.switch_to_quotes *)
+
+unbundle Hybrid_Program_Syntax
+
+declare [[literal_variables=false]]
+
+lemma fbox_kstarI:
+  assumes "I s" "\<And> s\<^sub>0. I s\<^sub>0 \<Longrightarrow> fbox C I s\<^sub>0" "\<And> s\<^sub>0. I s\<^sub>0 \<Longrightarrow> Q s\<^sub>0" 
+  shows "fbox (C\<^sup>*) Q s"
+  by (metis (mono_tags, opaque_lifting) SEXP_def assms(1,2,3) fbox_iso fbox_kstar_inv
+      le_bool_def le_funD predicate1I)
+
+
+lemma hl_pre_ghost: 
+  assumes "\<And> x. H{\<guillemotleft>x\<guillemotright> = e \<and> P} C {Q}"
+  shows "H{P} C {Q}"
+  using assms by fastforce
+
+lemma hl_middle_state:
+  assumes "\<And> x. H{P} C\<^sub>1 {\<guillemotleft>x\<guillemotright> = e \<longrightarrow> @(I x)}" "\<And> x. H{\<guillemotleft>x\<guillemotright> = e \<and> @(I x)} C\<^sub>2 {Q}"
+  shows "H{P} C\<^sub>1 ; C\<^sub>2 {Q}"
+  using assms 
+  apply (simp add: fbox_kcomp)
+  apply (auto simp add: fbox_def SEXP_def)
+  using le_bool_def le_funD by fastforce
+
+declare [[literal_variables]]
 
 notation norm ("\<parallel>_\<parallel>")
 notation infnorm ("\<parallel>_\<parallel>\<^sub>\<infinity>")
@@ -31,7 +59,7 @@ dataspace obstacle_avoidance =
   variables
     t :: real
     p :: "real ^ 2"
-    s :: real
+    sp :: real
     a :: real
     \<omega> :: real
     d :: "real ^ 2"
@@ -46,17 +74,17 @@ begin
 definition ctrl :: "'st prog \<Rightarrow> ('st \<Rightarrow> bool) \<Rightarrow> 'st prog" where
   "ctrl drive safe = 
     (a := -b
-     \<sqinter> \<questiondown>s = 0? ; a := 0 ; \<omega> := 0
-     \<sqinter> drive ; \<omega> := ? ; \<questiondown>-\<Omega> \<le> \<omega> \<and> \<omega> \<le> \<Omega>? ; r := ? ; \<questiondown>r \<noteq> 0 \<and> r * \<omega> = s \<and> @safe?) ;
+     \<sqinter> \<questiondown>sp = 0? ; a := 0 ; \<omega> := 0
+     \<sqinter> drive ; \<omega> := ? ; \<questiondown>-\<Omega> \<le> \<omega> \<and> \<omega> \<le> \<Omega>? ; r := ? ; \<questiondown>r \<noteq> 0 \<and> r * \<omega> = sp \<and> @safe?) ;
     t := 0"
 
-expression safe is "\<parallel>p - ob\<parallel>\<^sub>\<infinity> > (s\<^sup>2 / (2*b)) + (A/b + 1) * (A/2 * \<epsilon>\<^sup>2 + \<epsilon> * s)"
+expression safe is "\<parallel>p - ob\<parallel>\<^sub>\<infinity> > (sp\<^sup>2 / (2*b)) + (A/b + 1) * (A/2 * \<epsilon>\<^sup>2 + \<epsilon> * sp)"
 
 definition 
- "\<Psi> opc obc ac osc =
-  (ob = obc \<and> a = ac 
-    \<and> 0 \<le> s \<and> 0 \<le> t \<and> t \<le> \<epsilon> \<and> \<parallel>d\<parallel> = 1 \<and> s = osc + a * t
-    \<and> \<parallel>p - opc\<parallel>\<^sub>\<infinity> \<le> t * (s - a * t/2))\<^sup>e"
+ "\<Psi> = (\<lambda> (opc, obc, ac, osc).
+  (ob = obc \<and> a = ac
+    \<and> 0 \<le> sp \<and> 0 \<le> t \<and> t \<le> \<epsilon> \<and> \<parallel>d\<parallel> = 1 \<and> sp = osc + a * t
+    \<and> \<parallel>p - opc\<parallel>\<^sub>\<infinity> \<le> t * (sp - a * t/2))\<^sup>e)"
 
 expr_constructor \<Psi>
 
@@ -64,29 +92,49 @@ expression safety_condition is "0 < \<parallel>p - ob\<parallel>"
 
 notation safety_condition ("\<psi>")
 
-expression loop_invariant is "s^2/(2*b) < \<parallel>p - ob\<parallel>\<^sub>\<infinity> \<and> 0 \<le> s \<and> \<parallel>d\<parallel> = 1"
+expression loop_invariant is "sp^2/(2*b) < \<parallel>p - ob\<parallel>\<^sub>\<infinity> \<and> 0 \<le> sp \<and> \<parallel>d\<parallel> = 1"
 
 notation loop_invariant ("\<phi>")
 
-expression initial_condition is "s = 0 \<and> \<parallel>p - ob\<parallel>\<^sub>\<infinity> > 0 \<and> r \<noteq> 0 \<and> \<parallel>d\<parallel> = 1"
+expression initial_condition is "sp = 0 \<and> \<parallel>p - ob\<parallel>\<^sub>\<infinity> > 0 \<and> r \<noteq> 0 \<and> \<parallel>d\<parallel> = 1"
 
 notation initial_condition ("\<Phi>")
 
 definition dyn :: "'st prog" where
-"dyn = {t` = 1, p` = s *\<^sub>R d, s` = a, d` = \<omega> *\<^sub>R right_angle_rotation d, \<omega>` = a / r | s \<ge> 0 \<and> t \<le> \<epsilon>}"
+"dyn = {t` = 1, p` = sp *\<^sub>R d, sp` = a, d` = \<omega> *\<^sub>R right_angle_rotation d, \<omega>` = a / r | sp \<ge> 0 \<and> t \<le> \<epsilon>}"
 
 definition "model1 = (ctrl (a := A) safe ; dyn)\<^sup>*"
 
-lemma dyn_inv: "H{\<Psi> opc obc ac osc} dyn {\<Psi> opc obc ac osc}"
+lemma safety_from_Psi:
+  assumes "opc \<noteq> obc" "\<Psi> (opc, obc, 0, 0) s'"
+  shows "\<psi> s'"
+proof -
+  have "\<parallel>p<s'> - opc\<parallel>\<^sub>\<infinity> \<le> 0"
+    using assms by (auto simp add: \<Psi>_def safety_condition_def)
+  hence "\<parallel>p<s'> - opc\<parallel>\<^sub>\<infinity> = 0"
+    using infnorm_pos_le verit_la_disequality by blast
+  hence "p<s'> = opc"
+    by (meson eq_iff_diff_eq_0 infnorm_eq_0)
+  with assms have sep_eq:"\<parallel>p<s'> - ob<s'>\<parallel> = \<parallel>opc - obc\<parallel>"
+    by (simp add: \<Psi>_def)
+  from assms have old_sep: "0 < \<parallel>opc - obc\<parallel>"
+    by (simp add: \<Psi>_def)
+  show ?thesis
+    apply (simp add: safety_condition_def)
+    using old_sep sep_eq by force
+qed
+
+lemma dyn_inv: "H{\<Psi> (opc, obc, ac, osc)} dyn {\<Psi> (opc, obc, ac, osc)}"
   apply (unfold dyn_def \<Psi>_def)
   apply (dCut "\<parallel>d\<parallel> = 1")
    apply (invariant "d \<bullet> d = 1")
      apply dInduct_auto
      apply (smt (verit, ccfv_threshold) cross3_simps(36) inner_commute inner_real_def inner_scaleR_left right_angle_rotation_def)
     apply (simp add: norm_eq_1)
-  apply (simp add: norm_eq_1)
+   apply (simp add: norm_eq_1)
+  apply simp
   apply (dInduct_mega)
-  apply (invariant "- t * (s - a * t/2) \<le> (p - opc) $ 0 \<and> (p - opc) $ 0 \<le> t * (s - a * t/2) \<and> - t * (s - a * t/2) \<le> (p - opc) $ 1 \<and> (p - opc) $1 \<le> t * (s - a * t/2)")
+  apply (invariant "- t * (sp - a * t/2) \<le> (p - opc) $ 0 \<and> (p - opc) $ 0 \<le> t * (sp - a * t/2) \<and> - t * (sp - a * t/2) \<le> (p - opc) $ 1 \<and> (p - opc) $ 1 \<le> t * (sp - a * t/2)")
     apply (dInduct_mega)
   apply expr_simp
      apply (smt (verit) Finite_Cartesian_Product.norm_nth_le more_arith_simps(8) mult_left_le real_norm_def)
@@ -110,17 +158,110 @@ lemma ctrl_inv: "H{\<phi>} ctrl (a := A) safe {\<phi> \<and> t = 0}"
   apply wlp_simp
   done
 
+lemma fbox_choiceI:
+  assumes "fbox C\<^sub>1 P s" "fbox C\<^sub>2 P s"
+  shows "fbox (C\<^sub>1 \<sqinter> C\<^sub>2) P s"
+  by (metis (lifting) SEXP_def assms(1,2) fbox_choice)
+
+declare [[literal_variables=false]]
+
+lemma hl_fboxI: 
+  assumes "\<And> s. (P)\<^sub>e s \<Longrightarrow> fbox C (Q)\<^sub>e s"
+  shows "H{P} C {Q}"
+  using assms by blast
+
+lemma fboxI:
+  assumes "\<And> s'. \<lbrakk> s' \<in> C s \<rbrakk> \<Longrightarrow> P s'"
+  shows "fbox C P s"
+  by (simp add: assms fbox_def)
+
+lemma exec_assign: 
+  assumes "vwb_lens x" "\<And> s' x\<^sub>0. \<lbrakk> (get\<^bsub>x\<^esub> s' = e s); s = put\<^bsub>x\<^esub> s' x\<^sub>0 \<rbrakk> \<Longrightarrow> fbox C P s'" 
+  shows "fbox (x := e ; C) P s"
+  using assms 
+  by (simp add: fbox_def prog_defs expr_defs)
+     (metis mwb_lens_weak vwb_lens.put_eq vwb_lens_mwb weak_lens.put_get)
+
+declare [[literal_variables]]
+
 theorem static_safety: "H{\<Phi>} model1 {\<psi>}"
-  apply (unfold model1_def)
-  apply (kstar "loop_invariant")
-    apply (rule hoare_kcomp_inv)
-     defer
-     defer
-     apply expr_simp
-  apply expr_simp
-  apply (metis arith_simps(62) b_min divide_less_eq infnorm_eq_0 norm_le_zero_iff norm_pths(1)
-      power2_less_0 rel_simps(51) zero_compare_simps(6))
+proof (unfold model1_def, kstar "loop_invariant", simp add: ctrl_def loop_invariant_def safe_def, symbolic_exec, simp_all)
+  show "H{t = 0 \<and> \<omega> = 0 \<and> a = 0 \<and> sp\<^sup>2 / (2 * b) < \<parallel>p - ob\<parallel>\<^sub>\<infinity> \<and> 0 \<le> sp \<and> \<parallel>d\<parallel> = 1 \<and> sp = 0} 
+          dyn 
+         {sp\<^sup>2 / (2 * b) < \<parallel>p - ob\<parallel>\<^sub>\<infinity> \<and> 0 \<le> sp \<and> \<parallel>d\<parallel> = 1}"
+  proof (rule hl_fboxI, clarsimp)
+    fix s
+    assume t_0: "t<s> = 0" and \<omega>_0: "\<omega><s> = 0" and a_0: "a<s> = 0" and sep: "0 < \<parallel>p<s> - ob<s>\<parallel>\<^sub>\<infinity>" and d1: "\<parallel>d<s>\<parallel> = 1" and sp_0: "sp<s> = 0"
+    \<comment> \<open> We can show that the dynamics invariant holds initially \<close>
+    with eps_min have "\<Psi> (p<s>, ob<s>, a<s>, sp<s>) s"
+      by (simp add: \<Psi>_def infnorm_0)
+    show "( |dyn] (sp\<^sup>2 / (2 * b) < \<parallel>p - ob\<parallel>\<^sub>\<infinity> \<and> 0 \<le> sp \<and> \<parallel>d\<parallel> = 1)) s"
+    proof (intro fboxI, simp, safe)
+      fix s'
+      assume "s' \<in> dyn s"
+      have \<Psi>_s': "\<Psi> (p<s>, ob<s>, a<s>, sp<s>) s'"
+        by (smt (verit, best) SEXP_def \<open>\<Psi> (p<s>, ob<s>, a<s>, sp<s>) s\<close> \<open>s' \<in> dyn s\<close> dyn_inv
+            fbox_def predicate1D)
+      thus "(sp<s'>)\<^sup>2 / (2 * b) < \<parallel>p<s'> - ob<s'>\<parallel>\<^sub>\<infinity>"
+        by (simp add: \<Psi>_def, clarify)
+           (metis \<open>0 < \<parallel>p<s> - ob<s>\<parallel>\<^sub>\<infinity>\<close> \<open>a<s> = 0\<close> \<open>sp<s> = 0\<close> arith_simps(62,63) div_0
+            infnorm_pos_lt less_le_not_le nat_arith.rule0 power_zero_numeral
+            right_minus_eq)
+      from \<Psi>_s' sp_0 a_0 show "0 \<le> sp<s'>"
+        by (simp add: \<Psi>_def)
+      from \<Psi>_s' show "\<parallel>d<s'>\<parallel> = 1" by (simp add: \<Psi>_def)
+      have \<Psi>_s': "\<Psi> (p<s>, ob<s>, a<s>, sp<s>) s'"
+        by (smt (verit, best) SEXP_def \<open>\<Psi> (p<s>, ob<s>, a<s>, sp<s>) s\<close> \<open>s' \<in> dyn s\<close> dyn_inv
+            fbox_def predicate1D)
+    qed
+  qed
+next
+  show "H{t = 0 \<and> a = - b \<and> sp\<^sup>2 / (2 * b) < \<parallel>p - ob\<parallel>\<^sub>\<infinity> \<and> 0 \<le> sp \<and> \<parallel>d\<parallel> = 1} dyn
+         {sp\<^sup>2 / (2 * b) < \<parallel>p - ob\<parallel>\<^sub>\<infinity> \<and> 0 \<le> sp \<and> \<parallel>d\<parallel> = 1}"
+  proof (rule hl_fboxI, clarsimp)
+    fix s
+    assume t_0: "t<s> = 0" and a_b: "a<s> = - b" and sep: "(sp<s>)\<^sup>2 / (2 * b) < \<parallel>p<s> - ob<s>\<parallel>\<^sub>\<infinity>" and sp_pos: "0 \<le> sp<s>"
+           and d1: "\<parallel>d<s>\<parallel> = 1"
+    with eps_min have \<Psi>_s: "\<Psi> (p<s>, ob<s>, a<s>, sp<s>) s"
+      by (simp add: \<Psi>_def infnorm_0)
+    show "( |dyn] (sp\<^sup>2 / (2 * b) < \<parallel>p - ob\<parallel>\<^sub>\<infinity> \<and> 0 \<le> sp \<and> \<parallel>d\<parallel> = 1)) s"
+    proof (intro fboxI, simp, safe)
+      fix s'
+      assume "s' \<in> dyn s"
+      have \<Psi>_s': "\<Psi> (p<s>, ob<s>, a<s>, sp<s>) s'"
+        by (smt (verit, best) SEXP_def \<Psi>_s \<open>s' \<in> dyn s\<close> dyn_inv fbox_def predicate1D)
+      have hold: "sp<s> ^ 2 / (2 * b) < infnorm (p<s> - ob<s>)"
+        using sep by force
+      have hmove: "infnorm (p<s'> - p<s>) \<le> t<s'> * (sp<s> + -(b * t<s'>) - -(b * t<s'>) / 2)"
+      proof -
+        have hsp_eq: "sp<s'> = sp<s> + -(b * t<s'>)"
+          using \<Psi>_def \<Psi>_s' a_b minus_mult_right mult.commute prod.simps(2) by auto
+        show ?thesis
+          by (smt (verit) \<Psi>_def \<Psi>_s' hsp_eq prod.simps(2))
+      qed
+      have hgoal : "(sp<s> + -(b * t<s'>)) ^ 2 / (2 * b) < infnorm (p<s'> - ob<s>)"
+        sorry
+      thus "(sp<s'>)\<^sup>2 / (2 * b) < \<parallel>p<s'> - ob<s'>\<parallel>\<^sub>\<infinity>"
+      sorry
+(*
+    apply (rule hl_middle_state[where e="((p, ob, a, s))\<^sup>e" and I="\<Psi>"])
+     apply (simp add: ctrl_def safe_def loop_invariant_def \<Psi>_def)
+     apply wlp_simp
+     apply (smt (verit, del_insts) eps_min infnorm_0)
+  subgoal for vs
+    apply (case_tac vs)
+    subgoal for opc obc ac osc
+      apply (rule hoare_invI[where I="\<Psi> vs"])
+      apply simp
+      using dyn_inv apply auto[1]
+      apply simp
+    apply expr_auto
+     apply (simp add: ctrl_def safe_def loop_invariant_def \<Psi>_def)
+    apply expr_simp
+    apply auto[1]
   oops
+*)
+  
 
 end
 
